Traces.thy
@@ -1,78 +1,38 @@
+(*<*)
 theory Traces
-imports Main Transition_Systems
-begin
+imports Transition_Systems HML formula_prices_list HML_list
+begin    
+(*>*)
+
+subsection \<open>Trace semantics\<close>
 
 context lts
 begin
 
-inductive paths :: \<open>'s list \<Rightarrow> bool\<close> where
-  \<open>paths [p, p]\<close> |
-  \<open>paths (p#p'#ps)\<close> if \<open>\<exists>a. p \<mapsto> a p' \<and> paths (p'#ps)\<close>
-
-lemma
-  assumes \<open>paths (p # ps @ [p''])\<close>
-  shows \<open>\<exists>tr. p \<mapsto>$ tr p''\<close>
-  using assms
-proof (induct ps arbitrary: p)
-  case Nil
-  hence \<open>paths [p, p'']\<close>
-    by simp
-  hence \<open>p = p''\<close>
-    by (metis list.discI list.sel(1) list.sel(3) paths.cases)
-  hence \<open>p \<mapsto>$ [] p''\<close>
-    using step_sequence.intros(1) by blast
-  then show ?case
-    by blast
-next
-  case (Cons p' ps)
-  obtain a where \<open>p \<mapsto> a p'\<close> \<open>paths (p' # ps @ [p''])\<close>
-    using Cons.prems paths.simps[of \<open>p # (p' # ps) @ [p'']\<close>]
-    by auto
-  obtain tr where \<open>p' \<mapsto>$ tr p''\<close>
-    using Cons.hyps \<open>paths (p' # ps @ [p''])\<close>
-    by blast
-  then show ?case
-    using \<open>p \<mapsto> a p'\<close> step_sequence.intros(2)
-    by blast
-qed
-
-lemma
-  assumes \<open>p \<mapsto>$ tr p''\<close>
-  shows \<open>\<exists>ps. paths (p # ps @ [p''])\<close>
-  using assms
-proof (induct rule:step_sequence.induct)
-  case (1 p)
-  have \<open>paths (p # [] @ [p])\<close>
-    using paths.intros(1)
-    by simp
-  then show ?case by blast
-next
-  case (2 p a rt p'')
-  then show ?case
-    using paths.intros(2) append_Cons
-    by metis
-qed
-
-
+text \<open>As discussed, trace semantics identifies two processes as equal if they can perform the same set of action sequences.
+$\sigma \in \Act^* is a \textit{trace} of a process $p$ if there is a process $q$ such that $p\xrightarrow{\sigma}^*q$.
+Let $T(p)$ denote the set of traces of $p$.\<close>
 abbreviation traces :: \<open>'s \<Rightarrow> 'a list set\<close>
   where \<open>traces p \<equiv> {tr. \<exists>p'. p \<mapsto>$ tr p'}\<close>
+
+text \<open>Every process has the empty trace\<close>
 
 lemma empty_trace_trivial:
   fixes p
   shows \<open>[] \<in> traces p\<close>
   using step_sequence.intros by blast
 
-text \<open>Trace preorder as inclusion of trace sets\<close>
+text \<open>We say that $p$ is trace preordered by $q$ iff $T(p) \subset T(q)$.\<close>
 
 definition trace_preordered (infix \<open>\<lesssim>T\<close> 60) where
   \<open>p \<lesssim>T q \<equiv> traces p \<subseteq> traces q\<close>
 
-text \<open>Trace equivalence as mutual preorder\<close>
+text \<open>We can define trace equivalence as mutual preorder, which means that $p \sim_T q$ iff $T(p) = T(q)$.\<close>
 
 abbreviation trace_equivalent (infix \<open>\<simeq>T\<close> 60) where
   \<open>p \<simeq>T q \<equiv> p \<lesssim>T q \<and> q \<lesssim>T p\<close>
 
-text \<open>Trace preorder is transitive\<close>
+text \<open>Trace preorder is transitive.\<close>
 lemma trace_preorder_transitive:
   shows \<open>transp (\<lesssim>T)\<close>
   unfolding transp_def trace_preordered_def by blast
@@ -87,7 +47,113 @@ proof (rule equivpI)
     unfolding transp_def trace_preordered_def by blast
 qed
 
+text \<open>\textbf{Definition} The set $\mathcal{L}_T$ of trace formulas over Act is recursively defined by:
+\begin{align*}
+\bigwedge\varnothing\in \mathcal{L}_T\\
+\text{If } \varphi\in \mathcal{L}_T \text{ and }a\in\Act\text{ then } \langle a \rangle\varphi\in\mathcal{L}_T
+\end{align*}\<close>
+inductive hml_trace :: "('a, 's)hml \<Rightarrow> bool" where
+trace_tt: "hml_trace TT" |
+trace_conj: "hml_trace (hml_conj {} {} \<psi>s)"|
+trace_pos: "hml_trace (hml_pos \<alpha> \<phi>)" if "hml_trace \<phi>"
 
+definition hml_trace_formulas
+  where
+"hml_trace_formulas \<equiv> {\<phi>. hml_trace \<phi>}"
 
+text \<open>Two processes $p$ and $q$ are trace-equivalent, if they satisfy the same formulas in $\mathcal{L}_T$\<close>
+
+definition hml_trace_equivalent where
+"hml_trace_equivalent p q \<equiv> (\<forall> \<phi>. \<phi> \<in> hml_trace_formulas \<longrightarrow> (p \<Turnstile> \<phi>) \<longleftrightarrow> (q \<Turnstile> \<phi>))"
+
+text \<open>This definition allows for the construction of trace such as $(\langle a_1 \rangle \langle a_2 \rangle \ldots \langle a_n \rangle \textsf{T})$, which represents action sequences or traces.\<close>
+
+text \<open>\textbf{Proposition} The language of formulas with prices below $(\infty, 1, 0, 0, 0, 0)$ characterizes trace equivalence, that is
+for two processes $p$, $q$: 
+$(\forall\varphi \in \mathcal{O}_T. p \models \varphi \longleftrightarrow q \models \varphi) \longleftrightarrow (\forall\varphi \in \mathcal{L}_T. p \models \varphi \longleftrightarrow q \models \varphi)$\<close>
+
+definition expr_traces
+  where
+"expr_traces = {\<phi>. (less_eq_t (expr \<phi>) (\<infinity>, 1, 0, 0, 0, 0))}"
+
+definition expr_trace_equivalent 
+  where
+"expr_trace_equivalent p q \<equiv> (\<forall> \<phi>. \<phi> \<in> expr_traces \<longrightarrow> (p \<Turnstile> \<phi>) \<longleftrightarrow> (q \<Turnstile> \<phi>))"
+
+lemma expr_2_lb: "expr_2 f \<ge> 1"
+  by ((induction f), simp+)
+
+subsection \<open>The set of formulas with prices less then or equal to (\infty, 1, 0, 0, 0, 0) is a subset of the HML trace subset\<close>
+
+lemma trace_right: 
+  assumes "hml_trace \<phi>"
+  shows "(less_eq_t (expr \<phi>) (\<infinity>, 1, 0, 0, 0, 0))"
+  using assms
+proof(induct \<phi> rule:hml_trace.induct)
+  case trace_tt
+  then show ?case by simp
+next
+  case (trace_conj \<psi>s)
+  have "(expr_4 (hml_conj {} {} \<psi>s)) = 0"
+    using expr_4.simps Sup_enat_def by auto
+  then show ?case by auto
+next
+  case (trace_pos \<phi> \<alpha>)
+  then show ?case by simp
+qed
+
+subsection \<open>The HML trace set is a subset of the set of formulas with prices less then or equal to 
+(\<infinity>, 1, 0, 0, 0, 0)\<close>
+
+\<comment> \<open>The set induced by the coordinates (\<infinity>, 1, 0, 0, 0, 0) only includes empty conjunctions\<close>
+lemma HML_trace_conj_empty:
+  assumes A1: "less_eq_t (expr (hml_conj I J \<Phi>)) (\<infinity>, 1, 0, 0, 0, 0)" 
+  shows "I = {} \<and> J = {}"
+proof-
+  have "expr_2 (hml_conj I J \<Phi>) = 1 + Sup ((expr_2 \<circ> \<Phi>) ` I \<union> (expr_2 \<circ> \<Phi>) ` J)"
+    using formula_prices_list.expr_2_conj by blast
+  with assms have "... \<le> 1"
+    using expr.simps less_eq_t.simps
+    by simp
+  hence le_0: "Sup ((expr_2 \<circ> \<Phi>) ` I \<union> (expr_2 \<circ> \<Phi>) ` J) \<le> 0"
+    by simp
+  hence le_0: "\<forall>x \<in> ((expr_2 \<circ> \<Phi>) ` I). x \<le> 0" "\<forall>x \<in> ((expr_2 \<circ> \<Phi>) ` J). x \<le> 0"
+    using Sup_le_iff UnCI
+    by metis+
+  have "\<forall>x \<in> ((expr_2 \<circ> \<Phi>) ` I). x \<ge> 1" 
+    "\<forall>x \<in> ((expr_2 \<circ> \<Phi>) ` J). x \<ge> 1" using expr_2_lb
+    by fastforce+
+  with le_0 show ?thesis using imageI 
+    by simp
+qed
+
+lemma trace_left:
+  assumes "(less_eq_t (expr \<phi>) (\<infinity>, 1, 0, 0, 0, 0))"
+  shows "(hml_trace \<phi>)"
+  using assms
+proof(induction \<phi>)
+  case TT
+  then show ?case
+    using trace_tt by blast
+next
+  case (hml_pos \<alpha> \<phi>)
+  then show ?case 
+    using trace_pos by simp
+next
+  case (hml_conj I J \<Phi>)
+  then show ?case using HML_trace_conj_empty trace_conj
+    by metis
+qed
+
+lemma HML_trace_lemma: 
+"(hml_trace \<phi>) = (less_eq_t (expr \<phi>) (\<infinity>, 1, 0, 0, 0, 0))"
+  using trace_left trace_right by blast
+
+lemma "hml_trace_equivalent p q \<longleftrightarrow> expr_trace_equivalent p q"
+  unfolding hml_trace_equivalent_def expr_trace_equivalent_def expr_traces_def hml_trace_formulas_def
+  using HML_trace_lemma 
+  by blast
+
+text \<open>On Infinity...\<close>
 end
 end
