Correspondences.thy
@@ -1,0 +1,15 @@
+(*<*)
+theory Correspondences
+  imports 
+    Pure
+begin
+(*>*)
+
+chapter \<open>The Correspondences\<close>
+
+text \<open>- Proofs of the form $\{\varphi| \textsf{expr}(\varphi) \leq e_x\} = \mathcal{O}_e_x \equiv$ HML[$\Sigma$]$_X$
+- \<close>
+
+(*<*)
+end
+(*>*)
