Failure_traces.thy
@@ -1,0 +1,39 @@
+theory Failure_traces
+  imports Failures Transition_Systems HML formula_prices_list
+begin
+
+subsection \<open>Failure trace semantics\<close>
+
+text \<open>We can imagine the observer not only observing all traces of a system but also identifying scenarios where specific behavior is not possible. 
+For Failures in particular, the observer can distinguish between step-sequences based on what actions are possible in the resulting state. 
+Another way to think about Failures is that the process autonomously chooses an execution path, but only using a set of free are allowed actions.
+We want the failure formulas to represent either a trace (of the form $\langle a_1 \rangle\langle a_2\rangle...\langle a_n \rangle\textsf{T}$)
+or a failure pair, where some set of actions is not possible (so $\langle a_1 \rangle\langle a_2\rangle...\langle a_n \rangle\bigwedge \Phi$ with $$)\<close>
+
+text \<open>\textbf{Definition} The language $\mathcal{O}_F$ of failure-formulas is defined recursively:
+$$\langle a \rangle \varphi if \varphi \in \mathcal[O}_F | \bigwedge_{i\inI}\lnot\langle a \rangle \textsf{T}$$\<close>
+
+inductive hml_failure_trace :: "('a, 's)hml \<Rightarrow> bool" where
+"hml_failure_trace TT" |
+"hml_failure_trace (hml_pos \<alpha> \<phi>)" if "hml_failure_trace \<phi>" |
+"hml_failure_trace (hml_conj I J \<Phi>)" 
+  if "(\<Phi> ` I) = {} \<or> (\<exists>i \<in> \<Phi> ` I. \<Phi> ` I = {i} \<and> hml_failure_trace i)"
+     "\<forall>j \<in> \<Phi> ` J. \<exists>\<alpha>. j = (hml_pos \<alpha> TT) \<or> j = TT" 
+
+definition hml_failure_trace_formulas
+  where
+"hml_failure_trace_formulas \<equiv> {\<phi>. hml_failure_trace \<phi>}"
+
+definition expr_failure_trace
+  where
+"expr_failure_trace = {\<phi>. (less_eq_t (expr \<phi>) (\<infinity>, \<infinity>, \<infinity>, 0, 1, 1))}"
+
+context lts
+begin
+
+definition expr_failure_trace_equivalent 
+  where
+"expr_failure_trace_equivalent p q \<equiv> (\<forall> \<phi>. \<phi> \<in> expr_failure_trace \<longrightarrow> (p \<Turnstile> \<phi>) \<longleftrightarrow> (q \<Turnstile> \<phi>))"
+
+end
+end
