Two_nested_sim.thy
@@ -1,0 +1,51 @@
+theory Two_nested_sim
+imports Transition_Systems HML formula_prices_list
+begin
+
+subsection \<open>Failures semantics\<close>
+
+text \<open>We can imagine the observer not only observing all traces of a system but also identifying scenarios where specific behavior is not possible. 
+For Failures in particular, the observer can distinguish between step-sequences based on what actions are possible in the resulting state. 
+Another way to think about Failures is that the process autonomously chooses an execution path, but only using a set of free are allowed actions.
+We want the failure formulas to represent either a trace (of the form $\langle a_1 \rangle\langle a_2\rangle...\langle a_n \rangle\textsf{T}$)
+or a failure pair, where some set of actions is not possible (so $\langle a_1 \rangle\langle a_2\rangle...\langle a_n \rangle\bigwedge \Phi$ with $$)\<close>
+
+text \<open>\textbf{Definition} The language $\mathcal{O}_F$ of failure-formulas is defined recursively:
+$$\langle a \rangle \varphi if \varphi \in \mathcal[O}_F | \bigwedge_{i\inI}\lnot\langle a \rangle \textsf{T}$$\<close>
+
+inductive hml_2_nested_sim :: "('a, 's) hml \<Rightarrow> bool" 
+  where
+"hml_2_nested_sim TT" |
+"hml_2_nested_sim (hml_pos \<alpha> \<phi>)" if "hml_2_nested_sim \<phi>" |
+"hml_2_nested_sim (hml_conj I J \<Phi>)" 
+if "(\<forall>x \<in> (\<Phi> ` I). hml_2_nested_sim x) \<and> (\<forall>y \<in> (\<Phi> ` J). HML_simulation y)"
+
+definition hml_2_nested_sim_formulas where
+"hml_2_nested_sim_formulas \<equiv> {\<phi>. hml_2_nested_sim \<phi>}"
+
+definition expr_2_nested_sim
+  where
+"expr_2_nested_sim = {\<phi>. (less_eq_t (expr \<phi>) (\<infinity>, \<infinity>, \<infinity>, \<infinity>, \<infinity>, 1))}"
+
+context lts
+begin
+
+definition expr_2_nested_sim_equivalent
+  where
+"expr_2_nested_sim_equivalent p q \<equiv> (\<forall> \<phi>. \<phi> \<in> expr_2_nested_sim \<longrightarrow> (p \<Turnstile> \<phi>) \<longleftrightarrow> (q \<Turnstile> \<phi>))"
+
+text \<open>Failure Pairs\<close>
+
+abbreviation failure_pairs :: \<open>'s \<Rightarrow> ('a list \<times> 'a set) set\<close>
+  where
+\<open>failure_pairs p \<equiv> {(xs, F)|xs F. \<exists>p'. p \<mapsto>$ xs p' \<and> (initial_actions p' \<inter> F = {})}\<close>
+
+text \<open>Failure preorder and -equivalence\<close>
+
+definition failure_preordered (infix \<open>\<lesssim>F\<close> 60) where
+\<open>p \<lesssim>F q \<equiv> failure_pairs p \<subseteq> failure_pairs q\<close>
+
+abbreviation failure_equivalent (infix \<open>\<simeq>F\<close> 60) where
+\<open> p \<simeq>F q \<equiv> p \<lesssim>F q \<and> q \<lesssim>F p\<close>
+end
+end
